deps/poulet4/lib/P4automata/Benchmarks/NegativeProof.v
@@ -1,0 +1,119 @@
+Require Import Poulet4.P4automata.Benchmarks.ProofHeader.
+Require Import Poulet4.P4automata.Benchmarks.SimpleParsers.
+
+Notation A := OneZero.aut.
+Notation conf := (P4automaton.configuration (P4A.interp A)).
+
+Definition r_states :=
+  Eval vm_compute in (Reachability.reachable_states
+                        OneZero.aut
+                        200
+                        ParseOne.Start
+                        ParseZero.Start).
+
+Definition top : Relations.rel conf := fun _ _ => True.
+Definition top' : Relations.rel (state_template A) := fun _ _ => True.
+
+Declare ML Module "mirrorsolve".
+
+RegisterPrim (@TVar (sig A) (CEmp _) (Bits 0)) "p4a.core.var".
+RegisterPrim (@TFun (sig A) (CEmp _) [] (Bits 0)) "p4a.core.fun".
+
+RegisterPrim (@VHere (sig A) (CEmp _) (Bits 0)) "p4a.core.vhere".
+RegisterPrim (@VThere (sig A) (CEmp _) (Bits 0) (Bits 0)) "p4a.core.vthere".
+
+
+RegisterPrim (@FEq (sig A) (CEmp _) (Bits 0)) "p4a.core.eq".
+RegisterPrim (@FTrue (sig A) (CEmp _)) "p4a.core.tt".
+RegisterPrim (@FFalse (sig A) (CEmp _)) "p4a.core.ff".
+RegisterPrim (@FRel (sig A) (CEmp _)) "p4a.core.rel".
+RegisterPrim (@FNeg (sig A) (CEmp _)) "p4a.core.neg".
+RegisterPrim (@FOr (sig A) (CEmp _)) "p4a.core.or".
+RegisterPrim (@FAnd (sig A) (CEmp _)) "p4a.core.and".
+RegisterPrim (@FForall (sig A) (CEmp _)) "p4a.core.forall".
+
+RegisterPrim (@FImpl (sig A) (CEmp _)) "p4a.core.impl".
+
+RegisterPrim (@CEmp (sig A)) "p4a.core.cnil".
+RegisterPrim (@CSnoc (sig A)) "p4a.core.csnoc".
+
+RegisterPrim (@inl nat bool) "coq.core.inl".
+RegisterPrim (@inr nat bool) "coq.core.inr".
+
+RegisterPrim FirstOrderConfRelSimplified.Bits "p4a.sorts.bits".
+RegisterPrim FirstOrderConfRelSimplified.Store "p4a.sorts.store".
+
+RegisterPrim FirstOrderConfRelSimplified.BitsLit "p4a.funs.bitslit".
+RegisterPrim FirstOrderConfRelSimplified.Concat "p4a.funs.concat".
+RegisterPrim FirstOrderConfRelSimplified.Slice "p4a.funs.slice".
+RegisterPrim FirstOrderConfRelSimplified.Lookup "p4a.funs.lookup".
+
+RegisterPrim (@HList.HNil nat (fun _ => bool)) "p4a.core.hnil".
+RegisterPrim (@HList.HCons nat (fun _ => bool)) "p4a.core.hcons".
+
+RegisterEnvCtors 
+  (ParseOne.Bit, FirstOrderConfRelSimplified.Bits 1)  
+  (ParseZero.Bit, FirstOrderConfRelSimplified.Bits 1).
+
+(* These parsers are different, this proof should fail *)
+Lemma prebisim_negative:
+  pre_bisimulation A
+                   (wp r_states)
+                   top
+                   []
+                   [BCEmp, ⟨ inr false, 0 ⟩ ⟨ inr true, 0 ⟩ ⊢ bfalse;
+                    BCEmp, ⟨ inr true, 0 ⟩ ⟨ inr false, 0 ⟩ ⊢ bfalse]
+                   {| cr_st := {|
+                        cs_st1 := {|
+                          st_state := inl (inl (ParseOne.Start));
+                          st_buf_len := 0;
+                        |};
+                        cs_st2 := {|
+                          st_state := inl (inr (ParseZero.Start));
+                          st_buf_len := 0;
+                        |};
+                      |};
+                      cr_ctx := BCEmp;
+                      cr_rel := btrue;
+                   |}.
+Proof.
+
+  time "build phase" repeat (time "single step" run_bisim top top' r_states).
+
+  apply PreBisimulationClose.
+  
+  cbn.
+  unfold interp_entailment'.
+  simpl.
+  unfold top, interp_crel, interp_conf_rel'.
+  simpl.
+  unfold interp_conf_state.
+  simpl.
+  unfold interp_state_template.
+  simpl.
+  intros.
+  repeat match goal with 
+  | H: _ /\ _ |- _ => destruct H
+  end.
+  specialize (H1 tt).
+  autorewrite with interp_store_rel in H1.
+  cbn.
+  unfold interp_conf_rel.
+  simpl.
+  unfold interp_conf_state.
+  simpl.
+  unfold interp_state_template.
+  simpl.
+  split; [|split]. 
+
+  all: 
+    intros;
+    repeat match goal with 
+    | H: _ /\ _ |- _ => destruct H
+    end.
+  (* yikes, both of the goals here are contradictory... *)
+  - exfalso; congruence.
+  - exfalso; congruence.
+  - trivial.
+
+Time Admitted.
