deps/poulet4/lib/P4automata/Benchmarks/SimpleParsers.v
@@ -1,0 +1,208 @@
+Require Coq.Classes.EquivDec.
+Require Coq.Lists.List.
+Import List.ListNotations.
+Require Import Coq.Program.Program.
+Require Import Poulet4.P4automata.Syntax.
+Require Import Poulet4.FinType.
+Require Import Poulet4.P4automata.Sum.
+
+Ltac prep_equiv :=
+  unfold Equivalence.equiv, RelationClasses.complement in *;
+  program_simpl; try congruence.
+
+Obligation Tactic := prep_equiv.
+
+Module ParseOne.
+  Inductive state :=
+  | Start.
+  Equations state_eq_dec (l: state) (r: state) : {l = r} + {l <> r} :=  
+  { state_eq_dec Start Start := left eq_refl }.
+
+  Global Instance state_eqdec: EquivDec.EqDec state eq := state_eq_dec.
+  Global Program Instance state_finite: @Finite state _ state_eq_dec :=
+    {| enum := [Start] |}.
+  Next Obligation.
+    repeat constructor;
+      repeat match goal with
+             | H: List.In _ [] |- _ => apply List.in_nil in H; exfalso; exact H
+             | |- ~ List.In _ [] => apply List.in_nil
+             | |- ~ List.In _ (_ :: _) => unfold not; intros
+             | H: List.In _ (_::_) |- _ => inversion H; clear H
+             | _ => discriminate
+             end.
+  Qed.
+  Next Obligation.
+    destruct x; intuition congruence.
+  Qed.
+
+  Inductive header : nat -> Type :=
+  | Bit : header 1.
+
+  Equations header_eqdec_ (n: nat) (x: header n) (y: header n) : {x = y} + {x <> y} :=
+  {
+    header_eqdec_ _ Bit Bit := left eq_refl ;
+  }.
+
+  Global Instance header_eqdec: forall n, EquivDec.EqDec (header n) eq := header_eqdec_.
+
+  Global Instance header_eqdec': EquivDec.EqDec (Syntax.H' header) eq.
+  Proof.
+    solve_eqdec'.
+  Defined.
+
+  Global Instance header_finite: forall n, @Finite (header n) _ _.
+  Proof.
+    intros n; solve_indexed_finiteness n [1].
+  Qed.
+
+  Global Program Instance header_finite': @Finite {n & header n} _ header_eqdec' :=
+    {| enum := [ existT _ _ Bit] |}.
+  Next Obligation.
+    repeat constructor;
+    unfold "~";
+    intros;
+    destruct H;
+    now inversion H || now inversion H0.
+  Qed.
+  Next Obligation.
+  dependent destruction X; subst;
+  repeat (
+    match goal with
+    | |- ?L \/ ?R => (now left; trivial) || right
+    end
+  ).
+  Qed.
+
+  Definition states (s: state) :=
+    match s with
+    | Start =>
+      {| st_op := OpExtract (existT _ _ Bit);
+         st_trans := TSel (CExpr (EHdr Bit))
+                              [{| sc_pat := PExact (VBits 1 (tt, true));
+                                  sc_st := inr (A := state) true |}]
+                              (inr false) |}
+    end.
+
+  Program Definition aut: Syntax.t state header :=
+    {| t_states := states |}.
+  Solve Obligations with (destruct s; cbv; Lia.lia).
+
+End ParseOne.
+
+Module ParseZero.
+  Inductive state :=
+  | Start.
+  Equations state_eq_dec (l: state) (r: state) : {l = r} + {l <> r} :=  
+  { state_eq_dec Start Start := left eq_refl }.
+
+  Global Instance state_eqdec: EquivDec.EqDec state eq := state_eq_dec.
+  Global Program Instance state_finite: @Finite state _ state_eq_dec :=
+    {| enum := [Start] |}.
+  Next Obligation.
+    repeat constructor;
+      repeat match goal with
+             | H: List.In _ [] |- _ => apply List.in_nil in H; exfalso; exact H
+             | |- ~ List.In _ [] => apply List.in_nil
+             | |- ~ List.In _ (_ :: _) => unfold not; intros
+             | H: List.In _ (_::_) |- _ => inversion H; clear H
+             | _ => discriminate
+             end.
+  Qed.
+  Next Obligation.
+    destruct x; intuition congruence.
+  Qed.
+
+  Inductive header : nat -> Type :=
+  | Bit : header 1.
+
+  Equations header_eqdec_ (n: nat) (x: header n) (y: header n) : {x = y} + {x <> y} :=
+  {
+    header_eqdec_ _ Bit Bit := left eq_refl ;
+  }.
+
+  Global Instance header_eqdec: forall n, EquivDec.EqDec (header n) eq := header_eqdec_.
+
+  Global Instance header_eqdec': EquivDec.EqDec (Syntax.H' header) eq.
+  Proof.
+    solve_eqdec'.
+  Defined.
+
+  Global Instance header_finite: forall n, @Finite (header n) _ _.
+  Proof.
+    intros n; solve_indexed_finiteness n [1].
+  Qed.
+
+  Global Program Instance header_finite': @Finite {n & header n} _ header_eqdec' :=
+    {| enum := [ existT _ _ Bit] |}.
+  Next Obligation.
+    repeat constructor;
+    unfold "~";
+    intros;
+    destruct H;
+    now inversion H || now inversion H0.
+  Qed.
+  Next Obligation.
+  dependent destruction X; subst;
+  repeat (
+    match goal with
+    | |- ?L \/ ?R => (now left; trivial) || right
+    end
+  ).
+  Qed.
+
+  Definition states (s: state) :=
+    match s with
+    | Start =>
+      {| st_op := OpExtract (existT _ _ Bit);
+         st_trans := TSel (CExpr (EHdr Bit))
+                              [{| sc_pat := PExact (VBits 1 (tt, false));
+                                  sc_st := inr (A := state) true |}]
+                              (inr false) |}
+    end.
+
+  Program Definition aut: Syntax.t state header :=
+    {| t_states := states |}.
+  Solve Obligations with (destruct s; cbv; Lia.lia).
+
+End ParseZero.
+
+Module OneZero.
+  Definition state: Type := Sum.S ParseOne.state ParseZero.state.
+  Global Instance state_eq_dec: EquivDec.EqDec state eq :=
+    ltac:(typeclasses eauto).
+
+  Definition header := Sum.H ParseOne.header ParseZero.header.
+  Global Instance header_eq_dec': EquivDec.EqDec (H' header) eq.
+  Proof.
+    eapply Sum.H'_eq_dec; typeclasses eauto.
+  Defined.
+
+  Global Instance header_eq_dec: forall n, EquivDec.EqDec (header n) eq.
+  Proof.
+    typeclasses eauto.
+  Defined.
+
+  Global Instance header_finite: forall n, @Finite (header n) _ (header_eq_dec n).
+  Proof.
+    typeclasses eauto.
+  Defined.
+
+  Global Instance header_finite': @Finite {n & header n} _ header_eq_dec'.
+  econstructor.
+  - eapply Sum.H_finite.
+  - intros.
+    simpl.
+    destruct x.
+    inversion h;
+    dependent destruction H;
+    dependent destruction h;
+    dependent destruction h;
+    repeat (
+      match goal with
+      | |- ?L \/ ?R => (now left; trivial) || right
+      end
+    ).
+  Defined.
+
+  Definition aut := Sum.sum ParseOne.aut ParseZero.aut.
+End OneZero.
